ironfleet/src/Dafny/Distributed/Protocol/RSL/FailureProof/Phase1/verify.sh
@@ -1,0 +1,25 @@
+#!/bin/bash -li
+
+# echo ""
+# echo "Verifying GenericLemmas.i.dfy"
+# dafny GenericLemmas.i.dfy | grep -iv "Warning"
+
+echo ""
+echo "Verifying Phase1Proof_helper0.i.dfy"
+dafny Phase1Proof_helper0.i.dfy | grep -iv "Warning"
+
+# echo ""
+# echo "Verifying Phase2Proof_helper1.i.dfy"
+# dafny Phase2Proof_helper1.i.dfy | grep -iv "Warning"
+
+# echo ""
+# echo "Verifying Phase2Proof_helper2.i.dfy"
+# dafny Phase2Proof_helper2.i.dfy | grep -iv "Warning"
+
+echo ""
+echo "Verifying Phase1Proof.i.dfy"
+dafny Phase1Proof.i.dfy | grep -iv "Warning"
+
+echo ""
+echo "Verifying Phase1Proof_toplevel.i.dfy"
+dafny Phase1Proof_toplevel.i.dfy | grep -iv "Warning"
